---
output:
  pdf_document: default
  html_document: default
---

# Deeper sampling [under construction]

## Deeper Dive: Sampling Distributions (Unequal population means)

## Previously

In the last chapter, we examined the scenario where there was distribution of sample means where the sample means differed due to random sampling only. We created a scenario where the sample means differed to random sampling only when we created three populations with identical means (and variances). This situation is depicted in the scenario below.

```{r sim3poprepeat, out.width = "100%", echo=FALSE, fig.cap= "Sampling from three populations with the same mean (and variance)"}
knitr::include_graphics("ch_deeper_sampling/images/pop_equal_means.png")
```

| Population |  Mean        | Variance        |
|:----------:|:------------:|:----------------|
| 1          | $\mu_{A1_{people}}= 172.50$ |  $\sigma_{1_{people}}^2= 156.3236$ |
| 2          | $\mu_{A2_{people}}= 172.50$ |  $\sigma_{2_{people}}^2= 156.3236$ |
| 3          | $\mu_{A3_{people}}= 172.50$ |  $\sigma_{3_{people}}^2= 156.3236$ |


We can think of there mean a mean of the population means:

$$
\begin{aligned} 
\mu_{\mu_A} &=  \frac{\sum{\mu_A}}{A} \\
&=  \frac{\mu_{A1}+\mu_{A2}+\mu_{A3}}{A} \\
&=  \frac{172.50 + 172.50 + 172.50}{3} \\
&= \frac{517.50}{3}\\
&= 172.50 \\
\end{aligned}
$$


$$
\begin{aligned} 
\sigma_{\mu_A}^2 &=  \frac{\sum (\mu_{A_i}-\mu_{\mu_A})^2}{A} \\
&=  \frac{(172.50 - 172.50)^2 + (172.50 - 172.50)^2 + (172.50 - 172.50)^2}{3} \\
&=  \frac{0}{3} \\
&=  0\\
\end{aligned}
$$




| Population |  Mean        | Variance        |
|:----------:|:------------:|:----------------|
| 1          | $\mu_{1_{people}}= 152.50$ |  $\sigma_{1_{people}}^2= 156.3236$ |
| 2          | $\mu_{2_{people}}= 172.50$ |  $\sigma_{2_{people}}^2= 156.3236$ |
| 3          | $\mu_{3_{people}}= 192.50$ |  $\sigma_{3_{people}}^2= 156.3236$ |

$$
\begin{aligned} 
\mu_{\mu_A} &=  \frac{\sum{\mu_A}}{A} \\
&=  \frac{\mu_{A1}+\mu_{A2}+\mu_{A3}}{A} \\
&=  \frac{152.50 + 172.50 + 192.50}{3} \\
&= \frac{517.50}{3}\\
&= 172.50 \\
\end{aligned}
$$


$$
\begin{aligned} 
\sigma_{\mu_A}^2 &=  \frac{\sum (\mu_{A_i}-\mu_{\mu_A})^2}{A} \\
&=  \frac{(152.50 - 172.50)^2 + (172.50 - 172.50)^2 + (162.50 - 172.50)^2}{3} \\
&=  \frac{20^2 + 0 + 20^2}{3} \\
&=  0\\
\end{aligned}
$$



$$
\sigma_{\bar{x}}^2= \frac{\sigma_{people}^2}{n} + \sigma_{\mu_A}^2
$$




Recall that when we c

|          Attribute           |                                  Parameter Calculation                                   |                               Estimate of Parameter                               | Reflects         |
|:----------------------------:|:----------------------------------------------------------------------------------------:|:---------------------------------------------------------------------------------:|:----------------:|
|      Method 1: Variance      |  $\sigma_{\bar{x}}^2 = \frac{\sum_{i=1}^{K=\infty}{(\bar{x}_i - \mu_{\bar{x}})^2}}{K}$   |    $s_{\bar{x}}^2 = \frac{\sum_{i=1}^{a}{(\bar{x}_i - \bar{\bar{x}})^2}}{a-1}$    | Sampling Error & Variance of Population Means |
|    Method 2 CLT: Variance    |                    $\sigma_{\bar{x}}^2 = \frac{\sigma_{people}^2}{n}$                    |                     $s_{\bar{x}}^2 = \frac{s_{people}^2}{n}$                      | Just Sampling Error |

